pulse/ulib/experimental/Steel.PCM.Reference.fst
@@ -22,6 +22,7 @@ open Steel.PCM.FractionalPermission
 open FStar.Ghost
 module H = Steel.PCM.HigherReference
 module U = FStar.Universe
+module A = Steel.PCM.Effect.Atomic
 module Basics = Steel.PCM.SteelT.Basics
 
 let ref a = H.ref (U.raise_t a)
@@ -30,46 +31,9 @@ let pts_to r p v = H.pts_to r p (hide (U.raise_val (reveal v)))
 
 let alloc x = H.alloc (U.raise_val x)
 
-
-assume
-val sl_admit (#a:_) (#p:_) (q:a -> slprop)
-  : SteelT a p q
-
-
 assume
 val sl_admit_atomic (#a:_) (#uses:_) (#p:_) (o:_) (q:a -> slprop)
   : SteelAtomic a uses o p q
-
-
-assume
-val elim_h_exists (#a:_) (p:a -> slprop) (q:slprop { forall m (x:a). interp (p x) m ==> interp q m} )
-  : SteelT unit (h_exists p)
-                (fun _ -> q)
-
-let lift_q #a (q:a -> slprop) : U.raise_t a -> slprop = fun v -> q (U.downgrade_val v)
-
-let lift_h_exists (#a:_) (p:a -> slprop)
-  : SteelT unit (h_exists p)
-                (fun _ -> h_exists #(U.raise_t a) (lift_q p))
-  = sl_admit _
-
-let h_exists_cong (#a:_) (p:a -> slprop) (q:a -> slprop {forall x. equiv (p x) (q x) })
-  : SteelT unit (h_exists p)
-                (fun _ -> h_exists q)
-  = sl_admit _
-
-module A = Steel.PCM.Effect.Atomic
-let lift_h_exists_atomic (#a:_) #u (p:a -> slprop)
-  : SteelAtomic unit u unobservable
-                (h_exists p)
-                (fun _a -> h_exists #(U.raise_t a) (lift_q p))
-  = sl_admit_atomic unobservable _
-
-let h_exists_cong_atomic (#a:_) #u (p:a -> slprop) (q:a -> slprop {forall x. equiv (p x) (q x) })
-  : SteelAtomic unit u unobservable
-                (h_exists p)
-                (fun _ -> h_exists q)
-  = sl_admit_atomic unobservable _
 
 let read r =
   let x = H.read r in
@@ -77,13 +41,13 @@ let read r =
 
 let read_refine #a #p q r =
   Basics.h_assert (h_exists (fun (v:a) -> pts_to r p v `star` q v));
-  lift_h_exists (fun (v:a) -> pts_to r p v `star` q v);
+  Basics.lift_h_exists (fun (v:a) -> pts_to r p v `star` q v);
   Basics.h_assert (h_exists (fun (v:U.raise_t a) -> pts_to r p (U.downgrade_val v) `star` q (U.downgrade_val v)));
-  h_exists_cong (fun (v:U.raise_t a) -> pts_to r p (U.downgrade_val v) `star` q (U.downgrade_val v))
-                (fun (v:U.raise_t a) -> H.pts_to r p v `star` lift_q q v);
-  Basics.h_assert (h_exists (fun (v:U.raise_t a) -> H.pts_to r p v `star` lift_q q v));
-  let x = H.read_refine (lift_q q) r in
-  Basics.h_assert (H.pts_to r p x `star` lift_q q x);
+  Basics.h_exists_cong (fun (v:U.raise_t a) -> pts_to r p (U.downgrade_val v) `star` q (U.downgrade_val v))
+                (fun (v:U.raise_t a) -> H.pts_to r p v `star` U.lift_dom q v);
+  Basics.h_assert (h_exists (fun (v:U.raise_t a) -> H.pts_to r p v `star` U.lift_dom q v));
+  let x = H.read_refine (U.lift_dom q) r in
+  Basics.h_assert (H.pts_to r p x `star` U.lift_dom q x);
   Basics.h_assert (pts_to r p (U.downgrade_val x) `star` q (U.downgrade_val x));
   Basics.return (U.downgrade_val x)
 
@@ -112,10 +76,10 @@ let ghost_read_refine #a #uses #p r q =
   lift_h_exists_atomic (fun (v:a) -> pts_to r p v `star` q v);
   A.h_assert_atomic (h_exists (fun (v:U.raise_t a) -> pts_to r p (U.downgrade_val v) `star` q (U.downgrade_val v)));
   h_exists_cong_atomic (fun (v:U.raise_t a) -> pts_to r p (U.downgrade_val v) `star` q (U.downgrade_val v))
-                       (fun (v:U.raise_t a) -> H.pts_to r p v `star` lift_q q v);
-  A.h_assert_atomic (h_exists (fun (v:U.raise_t a) -> H.pts_to r p v `star` lift_q q v));
-  let x = H.ghost_read_refine r (lift_q q) in
-  A.h_assert_atomic (H.pts_to r p x `star` lift_q q x);
+                       (fun (v:U.raise_t a) -> H.pts_to r p v `star` U.lift_dom q v);
+  A.h_assert_atomic (h_exists (fun (v:U.raise_t a) -> H.pts_to r p v `star` U.lift_dom q v));
+  let x = H.ghost_read_refine r (U.lift_dom q) in
+  A.h_assert_atomic (H.pts_to r p x `star` U.lift_dom q x);
   A.h_assert_atomic (pts_to r p (U.downgrade_val x) `star` q (U.downgrade_val x));
   A.return_atomic (U.downgrade_val x)
 
